% AUTHOR1: Pranay pranayrs@bu.edu
% AUTHOR2: Saurabh ssingh02@bu.edu
% AUTHOR3: Kratesh kratesh@bu.edu

$$0 = \prod_{k=1}^{n}(1-\frac{1}{k^3}) < 1 < n^\frac{1}{n} < log(n) < (1+\frac{1}{n})^n <  \sqrt[3]{n} < \sum_{k=1}^{\log n}\frac{n}{3^k} <\frac{n}{4} < n^3 < n^9+n+2 < (n+1)^n < n^{n^n}  $$

We have assumed that the value is n is really large. Using large values of n and plotting them in th

$(a) def\ A(n):if (n == 0):return\ 1$

$else:return\ A(n-1) * A(n-1) * A(n-1)$

$T(n) = 1$ when $n=0$

$T(n) = 3*T(n-1) when\ n>0$

$T(n) = 3^k * T(n-k) + \frac{3^k-1}{2}*c_2$

$let\ k = n$

$T(n) = 3^n * T(0) + \frac{3^k-1}{2}*c_2$

$T(n) = 3^k * c_1 + \frac{3^k-1}{2}*c_2$

$\in \Theta(3^n)$

(b) $def\ B(n):if (n == 0):return\ 1$

$if (B(n//2) >= 5):return B(n//2) + 5$

$else:return\ 5$

$Ans.\ T(n) = c_1$ when $n=0$

$T(n) = c_2$ when $n=1$

$T(n) = 2*T(n/2) +c_3$ when $n>1$

$=T(n) = 2^k * T(\frac{n}{2^k}) + (2^k-1)*c_3$

$let\ k = log(n)$

$= n*T(1) + (n-1)c_3$

$= n*c_2 + (n-1)c_3$

$\in \Theta(n)$


$(c)def\ C(n):if (n <= 1):return\ 1$

$sum=0for ii in range(int(math.sqrt(n))):$

$sum +=C(int(math.sqrt(n)))return sum$

$Ans.\ T(0) = T(1) = c_1$

$T(n) = n^\frac{1}{2}*T(n^\frac{1}{2}) +c_2$

$= n^\frac{1}{2^k+1}*T(n^\frac{1}{2^k})+c_3$


$(e)\ Ans.\ T(0) = c_1; T(1)=c_2$

$T(n) = T(n-1) + 2*T(n-2) + c_3$

$\frac{2^k}$
